wip

src/sequential/ReorderFuture.v
@@ -61,14 +61,71 @@ Definition release_event (e: ThreadEvent.t): Prop :=
   | _ => False
   end.
 
-Variant lower_step {lang} (th0 th1: Thread.t lang): Prop :=
+Variant lower_step {lang} e (th0 th1: Thread.t lang): Prop :=
 | lower_step_intro
-    pf e
-    (STEP: Thread.step pf e th0 th1)
+    (STEP: Thread.step true e th0 th1)
     (NPROMISE: no_promise e)
     (NRELEASE: ~ release_event e)
     (MEM: lower_memory th1.(Thread.memory) th0.(Thread.memory))
 .
+
+Lemma write_lower_memory_lower prom0 mem0 loc from to msg prom1 mem1 kind
+      (PROMISE: Memory.write prom0 mem0 loc from to msg prom1 mem1 kind)
+      (LOWER: lower_memory mem1 mem0)
+  :
+    exists msg, kind = Memory.op_kind_lower msg.
+Proof.
+  inv PROMISE. inv PROMISE0; eauto.
+  { eapply Memory.add_get0 in MEM. des.
+    hexploit lower_memory_get_inv; eauto. i. des; clarify. }
+  { eapply Memory.split_get0 in MEM. des.
+    hexploit lower_memory_get_inv; try apply GET1; eauto. i. des; clarify. }
+  { eapply Memory.remove_get0 in MEM. des.
+    hexploit lower_memory_get; eauto. i. des; clarify. }
+Qed.
+
+Lemma lower_step_joined_memory lang (th0 th1: Thread.t lang) e views
+      (STEP: lower_step e th0 th1)
+      (LOCAL: Local.wf (Thread.local th0) (Thread.memory th0))
+      (SC: Memory.closed_timemap (Thread.sc th0) (Thread.memory th0))
+      (CLOSED: Memory.closed (Thread.memory th0))
+      (MEMORY: joined_memory views th0.(Thread.memory))
+      (VIEWS: wf_views views)
+      (RELEASED: joined_released views th0.(Thread.local).(Local.promises) th0.(Thread.local).(Local.tview).(TView.rel))
+  :
+    joined_memory views th1.(Thread.memory).
+Proof.
+Admitted.
+
+Lemma lower_step_joined_released lang (th0 th1: Thread.t lang) e views
+      (STEP: lower_step e th0 th1)
+      (LOCAL: Local.wf (Thread.local th0) (Thread.memory th0))
+      (SC: Memory.closed_timemap (Thread.sc th0) (Thread.memory th0))
+      (CLOSED: Memory.closed (Thread.memory th0))
+      (MEMORY: joined_memory views th0.(Thread.memory))
+      (VIEWS: wf_views views)
+      (RELEASED: joined_released views th0.(Thread.local).(Local.promises) th0.(Thread.local).(Local.tview).(TView.rel))
+  :
+    joined_released views th1.(Thread.local).(Local.promises) th1.(Thread.local).(Local.tview).(TView.rel).
+Proof.
+Admitted.
+
+Lemma lower_step_jthread_step lang (th0 th1: Thread.t lang) e views
+      (STEP: lower_step e th0 th1)
+      (LOCAL: Local.wf (Thread.local th0) (Thread.memory th0))
+      (SC: Memory.closed_timemap (Thread.sc th0) (Thread.memory th0))
+      (CLOSED: Memory.closed (Thread.memory th0))
+      (MEMORY: joined_memory views th0.(Thread.memory))
+      (VIEWS: wf_views views)
+      (RELEASED: joined_released views th0.(Thread.local).(Local.promises) th0.(Thread.local).(Local.tview).(TView.rel))
+  :
+    JThread.step true e th0 th1 views views.
+Proof.
+  hexploit lower_step_joined_memory; eauto. i.
+  hexploit lower_step_joined_released; eauto. i.
+  inv STEP. econs; auto; ss.
+  { inv STEP0; inv STEP; ss. inv LOCAL0; ss. }
+Qed.
 
 Variant lower_steps {lang} (th0 th1: Thread.t lang): Prop :=
 | lower_steps_intro
@@ -78,7 +135,7 @@ Variant lower_steps {lang} (th0 th1: Thread.t lang): Prop :=
 
 Lemma lower_steps_equiv lang (th0 th1: Thread.t lang)
   :
-    lower_steps th0 th1 <-> rtc lower_step th0 th1.
+    lower_steps th0 th1 <-> rtc (tau lower_step) th0 th1.
 Proof.
   split.
   { i. inv H. revert MEM. induction STEPS.
@@ -87,7 +144,7 @@ Proof.
   }
   { i. induction H.
     { econs; eauto. refl. }
-    { inv IHclos_refl_trans_1n. inv H. econs.
+    { inv IHclos_refl_trans_1n. inv H. inv TSTEP. econs.
       { econs; [|eauto]. econs.
         { econs; eauto. econs; eauto. }
         { destruct e; ss. }
@@ -113,15 +170,15 @@ Proof.
   eexists. esplits; eauto; try refl.
 Qed.
 
-Lemma step_split_pure lang (th0 th2: Thread.t lang) pf e views0 views2
-      (STEP: JThread.step pf e th0 th2 views0 views2)
+Lemma step_split_pure lang (th0 th2: Thread.t lang) e views0 views2
+      (STEP: JThread.step true e th0 th2 views0 views2)
       (NPROMISE: no_promise e)
       (NRELEASE: ~ release_event e)
       (MEM: th2.(Thread.memory) = th0.(Thread.memory))
   :
     exists th1,
       (<<PROMISES: joined_promise_steps th0 th1 views0 views2>>) /\
-      (<<LOWER: rtc lower_step th1 th2>>) /\
+      (<<LOWER: rtc (tau lower_step) th1 th2>>) /\
       (<<MEM: th1.(Thread.memory) = th2.(Thread.memory)>>) /\
       (<<SC: th1.(Thread.sc) = th2.(Thread.sc)>>).
 Proof.
@@ -145,22 +202,101 @@ Proof.
   subst. esplits.
   { econs. }
   { econs; [|econs]. econs; eauto.
-    rewrite MEM. refl. }
+    { econs; eauto. rewrite MEM. refl. }
+    { destruct e; ss. }
+  }
   { auto. }
   { auto. }
 Qed.
 
+Lemma memory_op_diff_only
+      mem0 loc from to msg mem1 kind
+      (WRITE: Memory.op mem0 loc from to msg mem1 kind)
+      loc' to' from' msg'
+      (SOME: Memory.get loc' to' mem1 = Some (from', msg'))
+  :
+    (exists from'' msg'',
+        (<<GET: Memory.get loc' to' mem0 = Some (from'', msg'')>>) /\
+        (<<MSG: Message.le msg' msg''>>)) \/
+    ((<<LOC: loc' = loc>>) /\
+     (<<TO: to' = to>>) /\
+     (<<FROM: from' = from>>) /\
+     (<<MSG: msg' = msg>>) /\
+     (<<NONE: Memory.get loc' to' mem0 = None>>)).
+Proof.
+  inv WRITE.
+  { erewrite Memory.add_o in SOME; eauto. des_ifs.
+    { right. ss. des; clarify. splits; auto.
+      eapply Memory.add_get0; eauto. }
+    { left. esplits; eauto. refl. }
+  }
+  { erewrite Memory.split_o in SOME; eauto. des_ifs.
+    { right. ss. des; clarify. splits; auto.
+      eapply Memory.split_get0 in SPLIT. des; auto. }
+    { left. ss. des; clarify. eapply Memory.split_get0 in SPLIT.
+      des; clarify. esplits; eauto. refl. }
+    { left. esplits; eauto. refl. }
+  }
+  { erewrite Memory.lower_o in SOME; eauto. des_ifs.
+    { ss. des; clarify. left. eapply lower_succeed_wf in LOWER; eauto.
+      des; eauto. }
+    { left. esplits; eauto. refl. }
+  }
+  { erewrite Memory.remove_o in SOME; eauto. des_ifs.
+    left. esplits; eauto. refl. }
+Qed.
+
+Definition views_mem_le
+           (mem0 mem1: Memory.t)
+           (views0 views1: Loc.t -> Time.t -> list View.t)
+           (tvw: TView.t): Prop :=
+  forall loc ts (NEQ: views1 loc ts <> views0 loc ts),
+    (<<NIL: views0 loc ts = []>>) /\
+    exists from val released,
+      (<<GET: Memory.get loc ts mem1 = Some (from, Message.concrete val (Some released))>>) /\
+      (<<NONE: Memory.get loc ts mem0 = None>>) /\
+      (<<VIEW: views1 loc ts = (View.join (tvw.(TView.rel) loc) (View.singleton_ur loc ts))
+                                 ::(all_join_views (View.singleton_ur loc ts) (views0 loc from))>>).
+
+Lemma write_tview_join_singleton tvw sc loc0 ts0 ord loc1 ts1
+      (ORD: ~ Ordering.le Ordering.acqrel ord)
+      (TS: loc0 = loc1 -> Time.le ts0 ts1)
+  :
+    View.join (TView.rel (TView.write_tview tvw sc loc0 ts0 ord) loc1)
+              (View.singleton_ur loc1 ts1) =
+    View.join (TView.rel tvw loc1) (View.singleton_ur loc1 ts1).
+Proof.
+  ss. des_ifs. setoid_rewrite LocFun.add_spec; eauto.
+  destruct (LocSet.Facts.eq_dec loc1 loc0).
+  { subst. rewrite View.join_assoc. f_equal.
+    rewrite singleton_ur_join. f_equal.
+    apply TimeFacts.le_join_r. auto. }
+  { refl. }
+Qed.
+
+Local Opaque TView.write_tview.
+
 Lemma step_split lang (th0 th2: Thread.t lang) pf e views0 views2
       (STEP: JThread.step pf e th0 th2 views0 views2)
       (NRELEASE: ~ release_event e)
+      (LOCAL: Local.wf (Thread.local th0) (Thread.memory th0))
+      (SC: Memory.closed_timemap (Thread.sc th0) (Thread.memory th0))
+      (CLOSED: Memory.closed (Thread.memory th0))
+      (CONS: Local.promise_consistent th2.(Thread.local))
+      (MEMORY: joined_memory views0 th0.(Thread.memory))
+      (VIEWS: wf_views views0)
+      (RELEASED: joined_released views0 th0.(Thread.local).(Local.promises) th0.(Thread.local).(Local.tview).(TView.rel))
   :
     exists th1,
       (<<PROMISES: joined_promise_steps th0 th1 views0 views2>>) /\
-      (<<LOWER: rtc lower_step th1 th2>>) /\
+      (<<LOWER: rtc (tau lower_step) th1 th2>>) /\
       (<<MEM: th1.(Thread.memory) = th2.(Thread.memory)>>) /\
       (<<SC: th1.(Thread.sc) = th2.(Thread.sc)>>).
 Proof.
-  dup STEP. inv STEP. inv STEP1.
+  dup STEP. inv STEP.
+  assert (VIEWSLE0: views_le views0 views2).
+  { ii. apply NNPP. ii. hexploit VIEWSLE; eauto. i. des; ss. }
+  inv STEP1.
   { inv STEP. esplits.
     { econs; [|econs]. econs; eauto.
       { econs. econs; eauto. }
@@ -169,43 +305,127 @@ Proof.
     { ss. }
     { ss. }
   }
-  { inv STEP. inv LOCAL; ss.
+  { inv STEP. inv LOCAL0; ss.
     { eapply step_split_pure; eauto; ss. }
     { eapply step_split_pure; eauto; ss. }
-    { inv LOCAL0. ss. inv WRITE. esplits.
+    { inv LOCAL1. ss. dup WRITE. inv WRITE. esplits.
       { econs; [|econs]. econs.
         { econs. econs; ss. econs.
           { eauto. }
-          { admit. }
+          { econs; ss. eapply TViewFacts.op_closed_released; eauto.
+            { eapply LOCAL. }
+            { eapply Memory.write_op; eauto. }
+          }
           { ss. }
         }
-        { i. clarify. admit. }
-        { i. ss. hexploit VIEWSLE; eauto. i. des. splits; auto.
-          esplits; eauto. rewrite VIEW.
-          admit.
+        { i. clarify. unfold TView.write_released in *.
+          destruct (Ordering.le Ordering.relaxed ord) eqn:ORD0; econs.
+          inv MEMORY0. hexploit (COMPLETE loc0 to0).
+          { eapply Memory.write_get2 in WRITE0. des; eauto. }
+          rewrite View.join_bot_l. ss.
+          replace (Ordering.le Ordering.acqrel ord) with false in *.
+          2:{ destruct ord; ss. }
+          i. des. auto.
+        }
+        { i. ss.
+          hexploit VIEWSLE; eauto. i. des.
+          assert (ts = to).
+          { eapply Memory.promise_op in PROMISE0.
+            eapply memory_op_diff_only in PROMISE0; eauto. des; clarify. }
+          subst. esplits; eauto.
+          rewrite write_tview_join_singleton in VIEW; eauto.
+          { destruct ord; ss. }
+          { i. refl. }
         }
         { auto. }
         { auto. }
-        { ss. admit. }
+        { ss. ii. eapply Memory.promise_op_promise in PROMISE0. dup GET.
+          eapply memory_op_diff_only in GET0; eauto. des; clarify.
+          { inv MSG. inv RELEASED1.
+            exploit RELEASED; eauto. i.
+            replace (views0 loc0 ts) with (views2 loc0 ts) in x; auto.
+            apply NNPP. ii. exploit VIEWSLE0; eauto. ii.
+            rewrite H0 in x. ss. }
+          { admit. }
+        }
       }
-      { econs; [|econs]. econs.
-
-          auto.
-
-
-
-
-          { econs.
-
-
-
-      admit. }
+      { admit. }
+      { ss. }
+      { ss. }
+    }
     { admit. }
     { eapply step_split_pure; eauto; ss. }
     { admit. }
     { eapply step_split_pure; eauto; ss. }
   }
 Admitted.
+
+
+
+Definition delayed
+           lang (st0 st1: Language.state lang) (lc0 lc1: Local.t)
+           (mem0: Memory.t)
+           (sc0: TimeMap.t)
+           (views0: Loc.t -> Time.t -> list View.t)
+           (fin: Messages.t): Prop
+  :=
+    forall (mem1: Memory.t)
+           (sc1: TimeMap.t)
+           (views1: Loc.t -> Time.t -> list View.t)
+           (MEM: Memory.closed mem1)
+           (FUTURE: Memory.future mem0 mem1)
+           (SCLE: TimeMap.le sc0 sc1)
+           (FINALIZED: fin <4= Messages.of_memory mem1)
+           (VIEWLE: views_le views0 views1)
+           (VIEWS: wf_views views1)
+           (JOINED: joined_memory views1 mem1)
+           (SC: Memory.closed_timemap sc1 mem1)
+           (LOCAL: Local.wf lc1 mem1),
+    exists mem1' lc1',
+      (<<LOCAL: Local.wf lc0 mem1>>) /\
+      (<<JOINED: joined_released views1 lc0.(Local.promises) lc0.(Local.tview).(TView.rel)>>) /\
+      (<<STEPS: rtc (tau (@pred_step (fun e => no_promise e /\ ~ release_event e) lang)) (Thread.mk _ st0 lc0 sc1 mem1) (Thread.mk _ st1 lc1' sc1 mem1')>>) /\
+      (<<LOCAL: lower_local lc1' lc1>>) /\
+      (<<MEM: lower_memory mem1' mem1>>)
+.
+
+Lemma delayed_current
+      lang (st: Language.state lang) lc
+      mem0 sc0 views0 fin
+  :
+    delayed _ st st lc lc mem0 sc0 views0 fin.
+Proof.
+Admitted.
+
+Lemma delayed_future
+      lang (st0 st1: Language.state lang) lc0 lc1
+      mem0 sc0 views0 fin0
+      mem1 sc1 views1 fin1
+      (MEM: Memory.future mem0 mem1)
+      (SC: TimeMap.le sc0 sc1)
+      (VIEWS: views_le views0 views1)
+      (FIN: fin0 <4= fin1)
+      (FINALIZED: fin1 <4= Messages.of_memory mem1)
+      (DELAYED: delayed _ st0 st1 lc0 lc1 mem0 sc0 views0 fin0)
+  :
+    delayed _ st0 st1 lc0 lc1 mem1 sc1 views1 fin1.
+Proof.
+Admitted.
+
+Lemma delayed_step
+      lang (st0 st1 st2: Language.state lang) lc0 lc1 lc2
+      mem1 sc1 views1 mem2 sc2 views2 fin
+      pf e
+      (STEP: JThread.step pf e (Thread.mk _ st1 lc1 sc1 mem1) (Thread.mk _ st2 lc2 sc2 mem2) views1 views2)
+      (NRELEASE: ~ release_event e)
+      (DELAYED: delayed _ st0 st1 lc0 lc1 mem1 sc1 views1 fin)
+  :
+    exists lc0',
+      (<<PROMISES: joined_promise_steps (Thread.mk _ st0 lc0 sc1 mem1) (Thread.mk _ st0 lc0' sc2 mem2) views1 views2>>) /\
+      (<<DELAYED: delayed _ st0 st2 lc0' lc2 mem2 sc2 views2 (fin \4/ committed mem1 lc1.(Local.promises) mem2 lc2.(Local.promises))>>).
+Proof.
+Admitted.
+
 
       lang (st0 st1: Language.state lang) (lc0 lc1: Local.t)
            (mem0: Memory.t)
